Admissibility conjectures progress

coq/lang/PSProperties.v
@@ -1,15 +1,21 @@
 Set Implicit Arguments.
 From Lang Require Import Util RuleGraphs.
 
-Module PSProperties(PS : ProofSystem).
-Include PS.
-Module Import RG := RuleGraph(PS). 
+Section PSProperties.
+Variable univ : universe.
+Variable ps : proof_system univ.
+
+Notation stmt := univ.(stmt).
+Notation valid_stmt := univ.(valid_stmt).
+
+Implicit Type s : stmt.
+Implicit Type rg : rule_graph ps.
 
 Definition derivable s :=
-  exists rg, derives rg s.
+  exists (rg : rule_graph ps), derives rg s.
 
 Definition acyc_derivable s :=
-  exists rg, ~ cyclic rg /\ derives rg s.
+  exists (rg : rule_graph ps), ~ cyclic rg /\ derives rg s.
 
 (* A statement is valid if 
    a graph exists where 
@@ -19,7 +25,7 @@ Definition acyc_derivable s :=
 *)
 Theorem sound_from_acyclic_graph :
   forall (s:stmt),
-  (exists rg, 
+  (exists (rg : rule_graph ps),
     derives rg s /\ 
     ~ cyclic rg /\
     rules_in_graph_sound rg
@@ -35,14 +41,14 @@ Qed.
 Definition relatively_complete :=
   forall (s : stmt),
   valid_stmt s ->
-  exists rg,
+  exists (rg : rule_graph ps),
   derives rg s /\ rules_in_graph_sound rg.
 
 
 Definition relatively_complete_acyclic :=
   forall (s : stmt),
   valid_stmt s ->
-  exists rg,
+  exists (rg : rule_graph ps),
   derives rg s /\ rules_in_graph_sound rg /\ 
   ~ cyclic rg.
 
@@ -55,34 +61,137 @@ Proof.
   introv [rg [_ H1]]. exists~ rg.
 Qed.
 
-Module PSExtend <: ProofSystem.
-  Parameter r : Type.
-  Parameter valid_r : list stmt -> stmt -> Prop.
+Section ExtendPSProperties.
+Variable r : Type.
+Variable r_inhab : Inhab r.
+Variable valid_r : list stmt -> stmt -> Prop.
 
-  Definition stmt := PS.stmt.
-  Definition liftable := PS.liftable.
-  Definition valid_stmt := PS.valid_stmt.
-
-  Open Scope type_scope.
-  Definition rule := PS.rule + r.
-
-  Definition valid_rule (rl : rule) (pre : list stmt) (c : stmt) : Prop :=
-    match rl with 
-    | inl rl => PS.valid_rule rl pre c 
+Definition extend_ps : proof_system univ :=
+  let liftable := ps.(liftable) in
+  let rule := (ps.(rule) + r)%type in
+  let valid_rule (rl : rule) (pre : list stmt) (c : stmt) := match rl with 
+    | inl rl => ps.(valid_rule) rl pre c 
     | inr rl => valid_r pre c
-    end.
-  
-End PSExtend.
+    end
+  in
+  @mk_ps univ liftable rule valid_rule.
+
+Definition extend_rg (rg : rule_graph ps) : rule_graph extend_ps.
+Proof.
+  pose (erg_rule := fun nd => match rg.(rg_rule) nd with
+    | Lift _ => Lift extend_ps
+    | Rule _ r => Rule extend_ps (inl r)
+  end).
+  assert (forall nd : rg.(rg_node), 
+    match erg_rule nd with
+    | Rule _ r => extend_ps.(valid_rule) r (List.map rg.(rg_conc) (rg.(rg_prems) nd)) (rg.(rg_conc) nd)
+    | Lift _ => extend_ps.(liftable) (rg.(rg_conc) nd) /\ (rg.(rg_prems) nd) = nil
+    end).
+  2 : refine (@mk_rg univ extend_ps rg.(rg_nodes) rg.(rg_conc) erg_rule rg.(rg_prems) H).
+  subst erg_rule. simpls. intros.
+  pose proof (H2 := rg_wf nd).
+  destruct (rg_rule nd) eqn:H; auto.
+Defined.
+
+Lemma extend_lift_validity (rg : rule_graph ps) :
+  graph_lift_valid rg ->
+  graph_lift_valid (extend_rg rg).
+Proof.
+  introv H1. 
+  intro.
+  specializes H1 nd.
+  destruct (rg_rule nd) eqn:H2; auto.
+  destruct (@rg_rule univ ps rg nd) eqn:H3; auto.
+  unfolds extend_ps. simpls.
+  rewrite H3 in H2. discriminate.
+Qed.
+
+Lemma extend_derives (rg : rule_graph ps) (s : stmt) :
+  derives rg s ->
+  derives (extend_rg rg) s.
+Proof.
+  introv [H1 H2].
+  split~. now apply extend_lift_validity.
+Qed.
+
+End ExtendPSProperties.
 
 End PSProperties.
 
-Module MorePSProperties(PS : ProofSystem).
-Include PS.
-Module Import RG := RuleGraph(PS). 
-Module Import PSP := PSProperties(PS).
-(* Parameter  *)
+Section MorePSProperties.
+Variable univ : universe.
+Variable ps : proof_system univ.
+
+Notation stmt := univ.(stmt).
+Notation valid_stmt := univ.(valid_stmt).
+
+Implicit Type s : stmt.
+Implicit Type rg : rule_graph ps.
+
+Variable r : Type.
+Variable r_inhab : Inhab r.
+Variable valid_r : list stmt -> stmt -> Prop.
+
+Lemma thm_extend_mono :
+  theorem ps ⊆ theorem (extend_ps ps r valid_r).
+Proof.
+  introv [rg H1].
+  unfold theorem.
+  unfold derivable.
+  exists (extend_rg r valid_r rg).
+  now apply extend_derives.
+Qed.
+
+Lemma acyc_thm_extend_mono :
+  acyc_theorem ps ⊆ acyc_theorem (extend_ps ps r valid_r).
+Proof.
+  introv [rg [H1 H2]].
+  exists (extend_rg r valid_r rg).
+  split~; now apply extend_derives.
+Qed.
+
+Definition admits := 
+  theorem (extend_ps ps r valid_r) ⊆ theorem ps.
+
+Definition acyc_admits := 
+  acyc_theorem (extend_ps ps r valid_r) ⊆ acyc_theorem ps.
+
+Lemma admits_characteristic :
+  (forall (prems : list stmt) (conc : stmt),
+    valid_rule (extend_ps ps r valid_r) (inr (arbitrary r_inhab)) prems conc ->
+      List.Forall (derivable ps) prems ->
+      (derivable ps) conc)
+  <-> admits.
+Proof.
+  split. {
+    intros.
+    unfold admits.
+    introv [rg [H1 H2]].
+    unfold theorem.
+    (* Print extend_ps. *)
+    exists* H2.
+    specializes H (List.map rg.(rg_conc) (rg.(rg_prems) nd)) x.
+    apply H.
+    + simpls.
+      remember (extend_ps ps r valid_r) as ext.
+      pose (ext.(valid_rule)).
+      subst.
+      unfolds extend_ps. simpls.
+      specializes P (inr (arbitrary r_inhab)).
+      unfolds 
+    unfolds extend_ps. simpls.
+    specializes H (List.map rg.(rg_conc) (rg.(rg_prems) nd)) x.
+    apply H.
+    + pose proof (H3 : ps.(valid_rule)). destruct rg. simpls.
+    
+    
+     destruct arbitrary. unfold r_inhab.
+    unfold derivable.
+    unfold derives.
+    destruct rg. simpls.
+    auto.
+  }
+Qed.
 
 
-(* Lemma thm_extend_mono (PS : ProofSystem) (r : Type) (valid_r : list PS.stmt -> PS.stmt -> Prop) 
-  : True.
-   *)
+(* Lemma admits_characteristic : locally_sound (derivable ps) ->  *)
