coq/lang/Nodes.v
@@ -1,0 +1,115 @@
+Set Implicit Arguments.
+From Lang Require Import Util.
+From Coq Require Import Structures.OrderedTypeEx.
+From Coq Require FSetList FSetFacts FSetProperties.
+
+Module Node <: UsualOrderedType.
+  Include Nat_as_OT.
+End Node.
+
+Notation node := Node.t.
+
+Module Import NodeSet := FSetList.Make(Node).
+Module NodeSetFacts := FSetFacts.Facts(NodeSet).
+Module NodeSetProperties := FSetProperties.Properties(NodeSet).
+
+Section Nodes.
+
+Variable dom : NodeSet.t.
+
+Definition dommem := {nd | NodeSet.In nd dom}.
+
+Definition nodelist := list dommem.
+
+Lemma nodelist_pigeon : 
+  forall (l : nodelist),
+  length l > cardinal dom ->
+  ~ List.NoDup l.
+Proof.
+  intros. intro.
+  assert (List.incl 
+    (List.map (@proj1_sig elt (fun nd => NodeSet.In nd dom)) l) 
+    (elements dom)
+  ). {
+    unfolds. intros. sort.
+    apply List.in_map_iff in H1.
+    exists* H1. destruct x. simpls. subst.
+    dup_hyp i.
+    rewrite NodeSetFacts.elements_iff in i0.
+    apply SetoidList.InA_alt in i0. exists* i0.
+    now subst.
+  }
+  apply (List.NoDup_incl_length) in H1.
+  { rewrite cardinal_1 in *.
+    rewrite List.map_length in H1.
+    rewrite length_datatypes_length in H.
+    contradict H. now rewrite ngt_as_le. }
+  destruct l.
+  { simpls. apply List.NoDup_nil. }
+  apply List.NoDup_cons.
+  { intro. simpls.
+    apply List.NoDup_cons_iff in H0 as (?&?).
+    contradict H0.
+    apply List.in_map_iff in H2. exists* H2.
+    apply eq_sig_hprop in H2. subst~.
+    intros. apply proof_irrelevance. }
+  apply nodup_inj.
+  2: { now apply List.NoDup_cons_iff in H0 as (?&?). }
+  unfolds. intros.
+  apply eq_sig_hprop; auto.
+  intros. apply proof_irrelevance.
+Qed.
+
+Lemma nodelist_pigeon' : 
+  forall (l : nodelist),
+  List.NoDup l ->
+  length l <= cardinal dom.
+Proof.
+  intros. contra H.
+  apply nodelist_pigeon. math.
+Qed.
+
+Fact nodelist_all_elems :
+  forall (l : nodelist),
+  length l = cardinal dom ->
+  List.NoDup l ->
+  forall (x:dommem),
+  List.In x l.
+Proof.
+  intros. destruct x as (e&Ie). sort.
+  rewrite cardinal_1 in H.
+  assert (List.incl (elements dom)
+    (List.map (@proj1_sig elt (fun nd => NodeSet.In nd dom)) l)).
+  {
+    apply List.NoDup_length_incl.
+    - apply nodup_inj; auto.
+      unfolds. intros.
+      apply eq_sig_hprop in H1. subst~.
+      intros. apply proof_irrelevance.
+    - rewrite <- H, List.map_length, length_datatypes_length.
+      auto.
+    - unfolds. intros. sort.
+      apply List.in_map_iff in H1.
+      exists* H1. destruct x. simpls. subst.
+      dup_hyp i.
+      rewrite NodeSetFacts.elements_iff in i0.
+      apply SetoidList.InA_alt in i0. exists* i0.
+      now subst.
+  }
+  specializes H1 e. specializes H1.
+  { apply elements_1 in Ie.
+    apply SetoidList.InA_alt in Ie.
+    exists* Ie. subst~. }
+  apply List.in_map_iff in H1.
+  exists* H1. destruct x. simpls.
+  subst. replace Ie with i.
+  auto. apply proof_irrelevance.
+Qed.
+
+End Nodes.
+
+Definition proj_into_subdom
+  (dom:t) (e:elt) (e':dommem dom) (H:e <> proj1_sig e') : 
+    dommem (remove e dom) :=
+  exist (fun e' => In e' (remove e dom)) (proj1_sig e') 
+    (@remove_2 dom e (proj1_sig e') H (proj2_sig e')).
